Start auth_prop library

new/proof/github_com/goose_lang/goose/testdata/examples/channel_search_replace.v
@@ -1,10 +1,153 @@
+From iris.base_logic.lib Require Import saved_prop ghost_map.
 From New.proof Require Export proof_prelude.
 From New.proof.github_com.goose_lang.goose.model.channel
   Require Import chan_au_base chan_au_send chan_au_recv simple.
-From New.proof Require Import time sync.
+From New.proof Require Import time sync tok_set.
 From New.generatedproof.github_com.goose_lang.goose.testdata.examples Require Import channel.
 
 Set Default Proof Using "Type".
+
+Section auth_prop.
+
+Class authPropG Σ :=
+  {
+    #[local] savedPred_inG :: savedPropG Σ;
+    #[local] gnameSet_inG :: ghost_mapG Σ gname ();
+  }.
+
+Context `{!authPropG Σ}.
+
+Definition own_aprop_auth γ (P : iProp Σ) (n : nat) : iProp Σ :=
+  ∃ gns,
+    "Hgns" ∷ ghost_map_auth γ 1 (gset_to_gmap () gns) ∗
+    "Hused" ∷ ([∗ set] γprop ∈ gns, ∃ Q, saved_prop_own γprop DfracDiscarded Q) ∗
+    "HimpliesP" ∷ (([∗ set] γprop ∈ gns, ∃ Q, saved_prop_own γprop DfracDiscarded Q ∗ ▷ Q) ∗-∗ ▷ P) ∗
+    "%Hn" ∷ ⌜ size gns = n ⌝.
+#[global] Opaque own_aprop_auth.
+#[local] Transparent own_aprop_auth.
+
+Definition own_aprop_frag γ (P : iProp Σ) (n : nat) : iProp Σ :=
+  ∃ gns,
+    "Hgns" ∷ ([∗ set] γprop ∈ gns, γprop ↪[γ] ()) ∗
+    "HimpliesP" ∷ (([∗ set] γprop ∈ gns, ∃ Q, saved_prop_own γprop DfracDiscarded Q ∗ ▷ Q) ∗-∗ ▷ P) ∗
+    "%Hn" ∷ ⌜ size gns = n ⌝.
+#[global] Opaque own_aprop_frag.
+#[local] Transparent own_aprop_frag.
+
+Definition own_aprop γ (P : iProp Σ) : iProp Σ := own_aprop_frag γ P 1.
+#[global] Opaque own_aprop.
+#[local] Transparent own_aprop.
+
+Lemma own_aprop_auth_alloc :
+  ⊢ |==> ∃ γ, own_aprop_auth γ True 0.
+Proof.
+  iMod (ghost_map_alloc ∅) as (γ) "[H _]".
+  iExists γ. unfold own_aprop_auth. iExists ∅.
+  rewrite gset_to_gmap_empty. iFrame. rewrite !big_sepS_empty //.
+  iModIntro. repeat iSplitL; try done; iIntros "_ "; done.
+Qed.
+
+Lemma own_aprop_auth_add γ P Q n :
+  ⊢ own_aprop_auth γ P n ==∗ own_aprop_auth γ (P ∗ Q) (S n) ∗ own_aprop γ Q.
+Proof.
+  iNamed 1.
+  iMod (saved_prop_alloc Q (DfracOwn 1)) as (γprop) "HQ"; first done.
+  destruct (decide (γprop ∈ gns)).
+  { iDestruct (big_sepS_elem_of_acc _ _ γprop with "Hused") as "[[% Hbad] _]"; first done.
+    iCombine "Hbad HQ" gives "[%Hbad _]". done. }
+  iMod (ghost_map_insert γprop () with "Hgns") as "[Hgns_auth Hgns']".
+  { rewrite lookup_gset_to_gmap_None //. }
+  rewrite -gset_to_gmap_union_singleton.
+  iMod (saved_prop_persist with "HQ") as "#HQ".
+  iModIntro. iSplitR "Hgns'".
+  { iFrame. assert ({[γprop]} ## gns) by set_solver.
+    repeat rewrite !big_sepS_union // !big_sepS_singleton. iFrame "∗#".
+    subst. rewrite size_union // size_singleton /=. iSplitL; last done.
+    iSplit.
+    - iIntros "[HQ' HPs]". iSpecialize ("HimpliesP" with "HPs"). iFrame.
+      iDestruct "HQ'" as (?) "[HQ' HQfact]". iCombine "HQ HQ'" gives "[_ H]".
+      iNext. iRewrite "H". iFrame.
+    - iIntros "[HPfact HQfact]". iSplitR "HPfact HimpliesP".
+      + iExists _; iFrame "#∗".
+      + by iApply "HimpliesP".
+  }
+  iExists {[ _ ]}. rewrite !big_sepS_singleton. iFrame. rewrite size_singleton.
+  iSplitL; last done. iSplit.
+  - iIntros "(% & HQ' & HQfact)". iCombine "HQ HQ'" gives "[_ Heq]".
+    iNext. iRewrite "Heq". iFrame.
+  - iIntros "?". iFrame "#∗".
+Qed.
+
+Lemma own_aprop_auth_agree γ P P' n :
+  ⊢ own_aprop_auth γ P n -∗ own_aprop_frag γ P' n -∗ (▷ P ∗-∗ ▷ P').
+Proof.
+  iNamed 1. iNamedSuffix 1 "'".
+  iDestruct (ghost_map_lookup_big with "Hgns [Hgns']") as "%Hsub".
+  { instantiate (1:=gset_to_gmap () gns0). rewrite big_sepM_gset_to_gmap. iFrame. }
+  apply subseteq_dom in Hsub. rewrite !dom_gset_to_gmap in Hsub.
+  apply set_subseteq_size_eq in Hsub as Heq; last lia. subst. clear Hn' Hsub.
+  iSplit.
+  - iIntros "HP". iApply "HimpliesP" in "HP". iApply "HimpliesP'" in "HP". iFrame.
+  - iIntros "HP'". iApply "HimpliesP'" in "HP'". iApply "HimpliesP" in "HP'". iFrame.
+Qed.
+
+End auth_prop.
+
+Section waitgroup_idiom.
+Context `{hG: heapGS Σ, !ffi_semantics _ _}.
+Context `{!globalsGS Σ} {go_ctx : GoContext}.
+Context `{!syncG Σ}.
+
+Record WaitGroup_join_names :=
+  {
+    wg : WaitGroup_names;
+    wg_added : gname;
+  }.
+
+Implicit Types γ : WaitGroup_join_names.
+
+Print auth_set_auth.
+AuthProp :
+
+  P : iProp
+  n, k : nat
+
+ own_auth P n
+ own_frag P k
+
+ own_frag P k ∗ own_frag P' k' -∗ own_frag (P ∗ P') (k + k')
+
+ own_auth P n ∗ own_frag P' n -∗ ▷(P ≡ P')
+ own_auth P n ∗ own_frag P' n -∗ own_auth P'' 0
+
+Definition wg_inv γ : iProp Σ :=
+  inv nroot (
+      ∃ ctr added done,
+        "Hwg_ctr" ∷ own_WaitGroup γ.(wg) ctr ∗
+        "Hadded" ∷ own_tok_auth_dfrac γ.(wg_added) (DfracOwn (1/2)) added ∗
+        "Hdone" ∷ own_tok_auth_dfrac γ.(wg_added) (DfracOwn (1/2)) done ∗
+        "" ∷ ⌜ uint.nat ctr = added + done ⌝
+    )
+.
+
+(** Permission to call `Add`. Calling `Add` will extend `A` with a caller-chosen
+    proposition, as long as `num_added` doesn't overflow. *)
+Definition own_Adder γ (num_added : w32) (P : iProp Σ) : iProp Σ :=
+  "Hno_waiters" ∷ own_WaitGroup_waiters γ.(wg) (W32 0)
+.
+
+(** Permission to call `Wait`, knowing that `P` will be true afterwards. *)
+Definition own_Waiter γ (P : iProp Σ) : iProp Σ :=
+  "Hwaiters" ∷ own_WaitGroup_waiters γ.(wg) (W32 1)
+.
+
+(** Permission to call `Done` as long as `P` is passed in. *)
+Definition own_Done γ (P : iProp Σ) : iProp Σ :=
+  True
+.
+
+
+End waitgroup_idiom.
 
 Section proof.
 Context `{hG: heapGS Σ, !ffi_semantics _ _}.
@@ -17,16 +160,46 @@ Context `{!chanGhostStateG Σ slice.t}.
 #[global] Instance : IsPkgInit chan_spec_raw_examples := define_is_pkg_init True%I.
 #[global] Instance : GetIsPkgInitWf chan_spec_raw_examples := build_get_is_pkg_init_wf.
 
+Record SearchReplace_names :=
+  {
+    wg: WaitGroup_names;
+    wg_added : gname;
+  }.
+
+Implicit Types γ : SearchReplace_names.
+
 Definition search_replace (x y: w64) : list w64 → list w64 :=
   fmap (λ a, if decide (a = x) then y else a).
 
+Definition wg_inv γ : iProp Σ :=
+  inv nroot (
+      ∃ ctr added done,
+        "Hwg_ctr" ∷ own_WaitGroup γ.(wg) ctr ∗
+        "Hadded" ∷ own_tok_auth_dfrac γ.(wg_added) (DfracOwn (1/2)) added ∗
+        "Hdone" ∷ own_tok_auth_dfrac γ.(wg_added) (DfracOwn (1/2)) done ∗
+        "" ∷ ⌜ uint.nat ctr = added + done ⌝
+    )
+.
+
+(* SearchReplace will own own_WaitGroup_waiters.
+   Invariant for counter will say
+ *)
 Definition chanP (x y: w64) (s: slice.t) : iProp Σ :=
   (* TODO: somehow this slice needs to be exactly the data in some subslice of
   the original list; does that need to be connected with a ghost variable? *)
-  ∃ (xs: list w64), s ↦* xs
+  ∃ (xs: list w64),
+    "Hxs" ∷ s ↦* xs ∗
+    "Hwg_done" ∷ (s ↦* (search_replace x y xs) ={⊤}=∗ own_wg_done_tok)
+.
   (* TODO: need permission to send back ownership of s ↦* search_replace x y
   xs on the waitgroup *)
 .
+
+
+Allocate
+(s ↦* (search_replace x y xs) ={⊤}=∗ own_wg_done_tok)
+(own_wg_done_tok ={⊤}=∗ s ↦* (search_replace x y xs))
+when calling Add.
 
 Definition waitgroupN := nroot .@ "waitgroup".
 
@@ -62,7 +235,7 @@ Proof.
     iApply "HΦ".
     iFrame.
   }
-  wp_apply wp_NewChannelRef.
+  wp_apply wp_NewChannel.
   { done. }
   iIntros (ch γch_names) "[#His_chan Hoc]".
   change (4 =? 0) with false; simpl.
